WIP on Fiat4Monitors example.

src/Fiat4Monitors/TurretMonitorSpec.v
@@ -1,81 +1,3 @@
-Require Import
-        Coq.Strings.String
-        Coq.Bool.Bool
-        Coq.Lists.List
-        Coq.Program.Program
-        Fiat.ADT
-        Fiat.ADTNotation
-        Fiat.ADTRefinement.
-
-Section RADL_Definitions.
-
-  Global Open Scope ADT_scope.
-  Global Open Scope string_scope.
-  Global Open Scope list_scope.
-  Global Open Scope ADTSig_scope.
-
-  Record RADL_Topic :=
-    { Topic_Name : string;
-      Topic_Type : Type }.
-
-  Variable Topics : list RADL_Topic. (* List of Topics in the Network. *)
-  Definition TopicID  := @BoundedString (map Topic_Name Topics).
-
-  Record RADL_Node :=
-    { (* Subscription + Publication info for this node *)
-      RADL_Subscriptions : list TopicID;
-      RADL_Publications : list TopicID
-    }.
-
-  Definition RADL_Init := "Init".
-  Definition RADL_Step := "Step".
-
-  Definition TopicTypes (topic : TopicID) : Type :=
-    Topic_Type (nth_Bounded Topic_Name Topics topic).
-
-  Definition Message topics := ilist TopicTypes topics.
-
-  Fixpoint SubMessage
-           (subtopics : list TopicID)
-           topics
-           (msg : Message topics)
-  : ilist TopicTypes subtopics :=
-    match subtopics return ilist TopicTypes subtopics with
-      | topic :: subtopics' =>
-        icons (B := TopicTypes) _ (ith_Bounded  msg topic) (SubMessage subtopics' msg)
-      | nil => inil _
-    end.
-
-  Definition RADL_ADTSig  (Node : RADL_Node)
-  : ADTSig :=                         (* A RADL Node is modeled as an ADT with a  *)
-    ADTsignature {                    (* single constructor and a step function. *)
-        Constructor RADL_Init      : unit -> rep,
-        Method      RADL_Step      : rep x ilist TopicTypes (RADL_Subscriptions Node)
-                                     -> rep x ilist TopicTypes (RADL_Publications Node)
-      }.
-
-  Definition RADL_ADTSpec (Node : RADL_Node)
-  : ADT (RADL_ADTSig Node) :=
-    ADTRep unit (* Since RADL Nodes are untrusted, we'll treat their state as completely unknown *)
-           { Def Constructor RADL_Init (_ : unit) : rep := ret tt,
-             Def Method RADL_Step (r : rep, in_t : ilist TopicTypes (RADL_Subscriptions Node)) : _ :=
-               (* Again, since the RADL Node is untrusted code, we'll assume that it can publish
-                  whatever the heck it wants. *)
-               results <- {out_t : ilist TopicTypes (RADL_Publications Node) | True };
-             ret (tt, results) }.
-
-  Definition RADLM_ADTSig
-             (Node MonitorNode : RADL_Node)
-             (InitDom : Type)
-  : ADTSig :=
-    ADTsignature {
-        Constructor RADL_Init      : InitDom -> rep,
-        Method      RADL_Step      : rep x unit * ilist TopicTypes (RADL_Subscriptions MonitorNode)
-                                     -> rep x unit * ilist TopicTypes (RADL_Publications MonitorNode)
-      }.
-
-End RADL_Definitions.
-
 Section Paintball.
 
   Require Bedrock.Platform.Facade.DFacade.
@@ -83,112 +5,214 @@ Section Paintball.
   Definition PaintballControlMode :=
     @BoundedString ["IDLE"; "SINGLE_SHOT"; "TRIPLE_SHOT"; "BURST"].
 
+  (* This is the list of topics available in the system.*)
   Definition PaintballTopics :=
     [ {| Topic_Name := "TiltX"; Topic_Type := Memory.W |};
       {| Topic_Name := "TiltY"; Topic_Type := Memory.W |};
       {| Topic_Name := "Trigger"; Topic_Type := PaintballControlMode |};
       {| Topic_Name := "Fired"; Topic_Type := PaintballControlMode |}].
 
+  (* Each RADL Node has a list of subscriptions and publications drawn
+     from the list of available topics. *)
   Definition BarrelNode : RADL_Node PaintballTopics :=
     {| RADL_Subscriptions := [ ``"Trigger"];
        RADL_Publications  := [ ``"Fired"] |}.
-
-  Definition BarrelSpec : Core.ADT (RADL_ADTSig BarrelNode) :=
-    RADL_ADTSpec BarrelNode.
-
   Definition TurretNode : RADL_Node PaintballTopics :=
     {| RADL_Subscriptions := [ ];
        RADL_Publications  := [``"TiltX"; ``"TiltY"] |}.
-
-  Definition TurretSpec : Core.ADT (RADL_ADTSig TurretNode) :=
-    RADL_ADTSpec TurretNode.
-
   Definition TriggerNode : RADL_Node PaintballTopics :=
     {| RADL_Subscriptions := [ ];
        RADL_Publications  := [ ``"Trigger"] |}.
 
+  (* Each RADL Node has a default implementation that nondeterministically
+     selects a publication value (since the underlying RADL Nodes are
+     untrusted code). *)
+  Definition BarrelSpec : Core.ADT (RADL_ADTSig BarrelNode) :=
+    RADL_ADTSpec BarrelNode.
+  Definition TurretSpec : Core.ADT (RADL_ADTSig TurretNode) :=
+    RADL_ADTSpec TurretNode.
   Definition TriggerSpec : Core.ADT (RADL_ADTSig TriggerNode) :=
     RADL_ADTSpec TriggerNode.
 
-  Definition PaintballSig :=
-    ADTsignature {
-        Constructor RADL_Init      : unit -> rep,
-        Method      RADL_Step      : rep x ilist Topic_Type PaintballTopics
-                                     -> rep x ilist (@TopicTypes PaintballTopics) [``"TiltX"; ``"TiltY"; ``"Trigger"; ``"Fired" ]
-      }.
+  Definition PaintballTopicIDs :=
+    RADL_Publications TurretNode ++ RADL_Publications TriggerNode ++ RADL_Publications BarrelNode.
 
+  (* Guard functions which check if the turret is pointed in a safe direction. *)
   Variables TiltXSafe TiltYSafe : Memory.W -> bool.
 
-  Notation GetTopic il idx := (ith_Bounded Topic_Name il ``idx).
-
-  Definition PaintballSpec : ADT PaintballSig :=
-    Eval simpl in ADTRep (unit * unit)
+  (* The complete specification is an ADT that has a single constructor that initializes the
+     RADL Nodes and a single step function that checks a global condition on each topic,
+     calling the original step functions if it holds and does some error handling otherwise. *)
+  Definition PaintballSpec :=
+    ADTRep (Rep BarrelSpec * Rep TurretSpec * Rep TriggerSpec)
                    { Def Constructor RADL_Init (_ : unit) : rep :=
                        barrel <- callCons BarrelSpec RADL_Init tt;
                        turret <- callCons TurretSpec RADL_Init tt;
                        trigger <- callCons TriggerSpec RADL_Init tt;
-                       ret (turret, trigger),
-                       Def Method RADL_Step (r : rep, in_t : ilist Topic_Type PaintballTopics) : _ :=
+                       ret (barrel, turret, trigger),
+
+                     Def Method RADL_Step (r : rep, in_t : Message PaintballTopicIDs) :
+                         (* Right now, we have a single, global guard that determines whether
+                            to call the original step functions. *)
+                       Message PaintballTopicIDs :=
                          if (TiltXSafe (GetTopic in_t "TiltX")
                                        && TiltYSafe (GetTopic in_t "TiltY")) then
-                           barrel <- callMeth BarrelSpec RADL_Step (snd r) (SubMessage (RADL_Subscriptions BarrelNode) in_t);
-                           turret <- callMeth TurretSpec RADL_Step (fst r) (SubMessage (RADL_Subscriptions TurretNode) in_t);
-                           trigger <- callMeth TriggerSpec RADL_Step (snd r) (SubMessage (RADL_Subscriptions TriggerNode) in_t);
-                           ret ((fst turret, fst trigger) ,
+                           (* Call the original step functions. *)
+                           barrel <- callMeth BarrelSpec RADL_Step (fst (fst r)) (SubMessage [````"Trigger" ] in_t);
+                           turret <- callMeth TurretSpec RADL_Step (snd (fst r)) (SubMessage [] in_t);
+                           trigger <- callMeth TriggerSpec RADL_Step (snd r) (SubMessage [] in_t);
+                           ret ((fst barrel, fst turret, fst trigger),
                                 (ilist_app (snd turret) (ilist_app (snd trigger) (snd barrel))))
                          else
-                           barrel <- callMeth BarrelSpec RADL_Step (snd r) (SubMessage (RADL_Subscriptions BarrelNode) in_t);
-                       turret <- callMeth TurretSpec RADL_Step (fst r) (SubMessage (RADL_Subscriptions TurretNode) in_t);
-                       ret ((tt, tt), (ilist_app (snd turret) (ilist_app
-                                                                 ((icons (B := @TopicTypes PaintballTopics)(``"Trigger") ``("IDLE") (inil _)))(snd barrel) )))}.
+                           (* The failure case calls the trigger and turret step functions
+                              and publishes "IDLE" for the barrel node. *)
+                           trigger <- callMeth TriggerSpec RADL_Step (fst (fst r)) (SubMessage [] in_t);
+                       turret <- callMeth TurretSpec RADL_Step (snd (fst r)) (SubMessage [] in_t);
+                       ret ((tt, fst turret, fst trigger),
+                            (ilist_app (snd turret) (ilist_app (snd trigger)
+                                                               ((icons (B := @TopicTypes PaintballTopics)(``"Fired") ``("IDLE") (inil _))))))}.
 
-  Definition TriggerMonitorNode : RADL_Node PaintballTopics :=
+  (* We now define the publication and subscription information for
+     and the specs of the monitor nodes. *)
+  Definition BarrelMonitorNode : RADL_Node PaintballTopics :=
     {| RADL_Subscriptions := [ ``"Trigger"; ``"TiltX"; ``"TiltY"];
-       RADL_Publications  := [ ] |}.
+       RADL_Publications  := [ ``"Fired"] |}.
 
   Definition TurretMonitorNode : RADL_Node PaintballTopics :=
     {| RADL_Subscriptions := [ ];
-       RADL_Publications  := [``"TiltX"; ``"TiltY"] |}.
+       RADL_Publications  := [ ``"TiltX"; ``"TiltY"] |}.
 
-  Definition TriggerMonitorSpec : Fiat.ADT.Core.ADT (RADLM_ADTSig TriggerNode TriggerMonitorNode unit).
-    refine (ADTRep unit
+  Definition TriggerMonitorNode : RADL_Node PaintballTopics :=
+    {| RADL_Subscriptions := [ ];
+       RADL_Publications  := [ ``"Trigger"] |}.
+
+  (* The specs distribute the global monitor to each monitor node.
+     In the case of the barrel, the monitor checks the turret position
+     before calling the original step function. *)
+  Definition BarrelMonitorSpec : Fiat.ADT.Core.ADT (RADLM_ADTSig BarrelMonitorNode unit) :=
+    ADTRep unit
            { Def Constructor RADL_Init (_ : unit) : rep := ret tt,
-             Def Method RADL_Step (r : rep, in_t : _) : _ := _}).
-    simpl in *.
-    refine (if (TiltXSafe (ilist_hd (ilist_tl (snd in_t)))
-                          && TiltYSafe (ilist_hd (ilist_tl (snd in_t)))) then
-              trigger <- callMeth TriggerSpec RADL_Step (fst in_t)
-                      (SubMessage (RADL_Subscriptions TriggerNode) (snd in_t))
-              ;
-              ret (tt, _)
-            else
-              ret (tt, _)).
-  Defined.
+             Def Method RADL_Step (r : rep, in_t : unit * Message (RADL_Subscriptions BarrelMonitorNode)) : _ :=
+               if (TiltXSafe (GetTopic (snd in_t) "TiltX")
+                             && TiltYSafe (GetTopic (snd in_t) "TiltY")) then
+                 barrel <- callMeth BarrelSpec RADL_Step (fst in_t)
+                         (SubMessage [````"Trigger" ] (snd in_t))
+                 ;
+                 ret (tt, barrel)
+               else
+                 ret (tt, (tt, (icons (B := @TopicTypes PaintballTopics)(``"Fired") ``("IDLE") (inil _))))
+           }.
 
-  Print TriggerMonitorSpec.
-
-  Definition TurretMonitorSpec : Fiat.ADT.Core.ADT (RADLM_ADTSig TurretNode TurretMonitorNode).
-    refine (ADTRep (RADL_Rep TurretMonitorNode)
+  (* The other two monitor nodes don't have to check anything to enforce the guard. *)
+  Definition TurretMonitorSpec : Fiat.ADT.Core.ADT (RADLM_ADTSig TurretNode unit) :=
+    ADTRep unit
            { Def Constructor RADL_Init (_ : unit) : rep := ret tt,
-             Def Method RADL_Step (r : rep, in_t : _) : _ :=
+             Def Method RADL_Step (r : rep, in_t : unit * Message (RADL_Subscriptions TurretMonitorNode)) : _ :=
                turret <- callMeth TurretSpec RADL_Step (fst in_t) (snd in_t);
-              ret (tt , turret)
+             ret (tt, turret)
+           }.
 
-           }).
+  Definition TriggerMonitorSpec : Fiat.ADT.Core.ADT (RADLM_ADTSig TriggerNode unit) :=
+    ADTRep unit
+           { Def Constructor RADL_Init (_ : unit) : rep := ret tt,
+             Def Method RADL_Step (r : rep, in_t : unit * Message (RADL_Subscriptions TriggerMonitorNode)) : _ :=
+               turret <- callMeth TriggerSpec RADL_Step (fst in_t) (snd in_t);
+             ret (tt, turret)
+           }.
+
+  (* After Refinement, we arrive at an implementation which simply calls the monitor functions,
+     with each function enforcing the global guard locally. *)
+  Definition PaintballImpl :
+  ADTRep (Rep BarrelMonitorSpec * Rep TriggerMonitorSpec *
+              Rep TurretMonitorSpec * Rep BarrelSpec *
+              Rep TriggerSpec * Rep TurretSpec)
+      { Def Constructor RADL_Init (_: ()) : rep :=
+          barrel <- (callCons BarrelSpec RADL_Init) ();
+          turret <- (callCons TurretSpec RADL_Init) ();
+          trigger <- (callCons TriggerSpec RADL_Init) ();
+          barrelmonitor <- (callCons BarrelMonitorSpec RADL_Init) ();
+          turretmonitor <- (callCons TurretMonitorSpec RADL_Init) ();
+          triggermonitor <- (callCons TriggerMonitorSpec RADL_Init) ();
+          ret
+            (barrelmonitor, turretmonitor, triggermonitor, barrel, turret,
+            trigger) ,
+        Def Method RADL_Step (r : rep, in_t : (Message PaintballTopicIDs)) :
+        (Message PaintballTopicIDs) :=
+          barrel <- (callMeth BarrelMonitorSpec RADL_Step)
+                      (snd r)
+                      ((),
+                      SubMessage
+                        [``(``("Trigger")); ``(``("TiltX")); ``(``("TiltY"))]
+                        in_t);
+          turret <- (callMeth TurretMonitorSpec RADL_Step)
+                      (snd r) ((), SubMessage [] in_t);
+          trigger <- (callMeth TriggerMonitorSpec RADL_Step)
+                       (snd r) ((), SubMessage [] in_t);
+          ret
+            (fst barrel, fst turret, fst trigger, fst (snd barrel),
+            fst (snd turret), fst (snd trigger),
+            ilist_app (snd (snd turret))
+              (ilist_app (snd (snd trigger)) (snd (snd barrel))))  })
+
+  (* This implementation includes a list of monitor node specs from which we
+     can derive Gallina implementations. Eventually (hopefully soon) we can
+     then plug these into our pipeline to produce Bedrock implementations which
+     can be integrated into the monitor framework. *)
 
   Definition PaintballImpl :
     MostlySharpened PaintballSpec.
   Proof.
     start sharpening ADT.
-    hone representation using (fun (r_o : RADL_Rep TurretNode *
-                                           RADL_Rep TriggerNode)
-                                      (r_n :
-                                          (RADL_Rep TriggerMonitorNode *
-                                           RADL_Rep TurretMonitorNode *
-                                           RADL_Rep TriggerNode *
-                                           RADL_Rep TurretNode))
-
+    hone representation using (fun (r_o : Rep PaintballSpec)
+                                   (r_n :
+                                      Rep BarrelMonitorSpec *
+                                      Rep TriggerMonitorSpec *
+                                      Rep TurretMonitorSpec *
+                                      Rep BarrelSpec *
+                                      Rep TriggerSpec *
+                                      Rep TurretSpec)
                                         => True).
+    { subst H.
+      instantiate (1 := fun d => barrel <- (callCons BarrelSpec RADL_Init) ();
+                   turret <- (callCons TurretSpec RADL_Init) ();
+                   trigger <- (callCons TriggerSpec RADL_Init) ();
+                   barrelmonitor <- (callCons BarrelMonitorSpec RADL_Init) ();
+                   turretmonitor <- (callCons TurretMonitorSpec RADL_Init) ();
+                   triggermonitor <- (callCons TriggerMonitorSpec RADL_Init) ();
+                   ret (barrelmonitor, turretmonitor, triggermonitor, barrel, turret, trigger)).
+      simplify with monad laws; refine pick val ( (), (), (), (), (), ()); eauto; simpl.
+      intros v Comp_v; computes_to_inv; subst; eauto.
+    }
+    {
+      subst H0; instantiate (1 := fun (r : Rep BarrelMonitorSpec *
+                                      Rep TriggerMonitorSpec *
+                                      Rep TurretMonitorSpec *
+                                      Rep BarrelSpec *
+                                      Rep TriggerSpec *
+                                      Rep TurretSpec)  (in_t : Message PaintballTopicIDs) =>
+              barrel <- callMeth BarrelMonitorSpec RADL_Step (snd r) (tt, (SubMessage [````"Trigger";
+                                                                                         ````"TiltX";
+                                                                                         ````"TiltY"] in_t));
+        turret <- callMeth TurretMonitorSpec RADL_Step (snd r) (tt, SubMessage [] in_t);
+        trigger <- callMeth TriggerMonitorSpec RADL_Step (snd r) (tt, SubMessage [] in_t);
+        ret ((fst barrel, fst turret, fst trigger, fst (snd barrel), fst (snd turret), fst (snd trigger)),
+             (ilist_app (snd (snd turret)) (ilist_app (snd (snd trigger)) (snd (snd barrel)))))).
+      simpl.
+      unfold eq_rect_r, eq_rect, eq_sym.
+      simpl.
+      admit.
+    }
+
+    simpl in H0.
+      simpl in c.
+      unfold methodType in H0.
+      simpl in H0.
+      unfold PaintballTopicIDs in H0.
+      simpl in H0.
+      eauto.
+    simpl; rewrite <- refineEquiv_bind_unit.
+    rewrite <- refineEquiv_bind_unit.
+    simplify with monad laws.
     simpl in *.
     unfold PaintballSpec.
 
