src/Fiat4Monitors/RADL_Definitions.v
@@ -1,0 +1,106 @@
+Require Import
+        Coq.Strings.String
+        Coq.Bool.Bool
+        Coq.Lists.List
+        Coq.Program.Program
+        Fiat.ADT
+        Fiat.ADTNotation
+        Fiat.ADTRefinement
+        Fiat.ADTRefinement.BuildADTRefinements.
+
+Section RADL_Definitions.
+
+  Global Open Scope ADT_scope.
+  Global Open Scope string_scope.
+  Global Open Scope list_scope.
+  Global Open Scope ADTSig_scope.
+
+  Record RADL_Topic :=
+    { Topic_Name : string;
+      Topic_Type : Type }.
+
+  Variable Topics : list RADL_Topic. (* List of Topics in the Network. *)
+  Definition TopicID  := @BoundedString (map Topic_Name Topics).
+
+  Record RADL_Node :=
+    { (* Subscription + Publication info for this node *)
+      RADL_Subscriptions : list TopicID;
+      RADL_Publications : list TopicID
+    }.
+
+  Definition RADL_Init := "Init".
+  Definition RADL_Step := "Step".
+
+  Definition TopicTypes
+             (topic : TopicID) : Type :=
+    Topic_Type (nth_Bounded Topic_Name Topics topic).
+
+  Definition Message topics :=
+    ilist TopicTypes topics.
+
+  Fixpoint SubTopic
+           (topics : list TopicID)
+           {struct topics}
+  : Message topics ->
+    forall (subtopic : BoundedIndex topics),
+      TopicTypes (bindex subtopic).
+  Proof.
+    refine (match topics return
+                  Message topics ->
+                  forall (subtopic : BoundedIndex topics),
+                    TopicTypes (bindex subtopic) with
+              | nil => fun msg subtopic => BoundedIndex_nil _ subtopic
+              | topic :: topics' =>  fun msg subtopic => _
+            end).
+    destruct subtopic as [idx [[ | n] nth_n]].
+    simpl in *; injection nth_n; intros; subst.
+    exact (ith_Bounded id msg {| bindex := _;
+                                indexb := Build_IndexBound (idx :: (map id topics')) 0 nth_n|}).
+    exact (SubTopic topics' (ilist_tl msg) {| bindex := idx;
+                       indexb := {| ibound := n;
+                                    boundi := nth_n |} |} ).
+  Defined.
+
+  Fixpoint SubMessage
+             (topics : list TopicID)
+             (subtopics : list (BoundedIndex  topics))
+             (msg : Message topics)
+  : Message (map (bindex (Bound := topics)) subtopics) :=
+    match subtopics return Message (map (bindex (Bound := topics)) subtopics) with
+      | nil => inil _
+      | subtopic :: subtopics' =>
+        icons _ (SubTopic msg subtopic )
+              (SubMessage subtopics' msg)
+    end.
+
+  Definition RADL_ADTSig  (Node : RADL_Node)
+  : ADTSig :=                         (* A RADL Node is modeled as an ADT with a  *)
+    ADTsignature {                    (* single constructor and a step function. *)
+        Constructor RADL_Init      : unit -> rep,
+        Method      RADL_Step      : rep x Message (RADL_Subscriptions Node)
+                                     -> rep x Message (RADL_Publications Node)
+      }.
+
+  Definition RADL_ADTSpec (Node : RADL_Node)
+  : ADT (RADL_ADTSig Node) :=
+    ADTRep unit (* Since RADL Nodes are untrusted, we'll treat their state as completely unknown *)
+           { Def Constructor RADL_Init (_ : unit) : rep := ret tt,
+             Def Method RADL_Step (r : rep, in_t : Message (RADL_Subscriptions Node)) : _ :=
+               (* Again, since the RADL Node is untrusted code, we'll assume that it can publish
+                  whatever the heck it wants. *)
+               results <- {out_t : Message (RADL_Publications Node) | True };
+             ret (tt, results) }.
+
+  Definition RADLM_ADTSig
+             (MonitorNode : RADL_Node)
+             (InitDom : Type)
+  : ADTSig :=
+    ADTsignature {
+        Constructor RADL_Init      : InitDom -> rep,
+        Method      RADL_Step      : rep x unit * Message (RADL_Subscriptions MonitorNode)
+                                     -> rep x unit * Message (RADL_Publications MonitorNode)
+      }.
+
+End RADL_Definitions.
+
+Notation GetTopic il idx := (SubTopic il ``(``idx)).
